added missing file

ver2/symbolic_state_cmp.v
@@ -96,6 +96,139 @@ unfold dummy_symbolic_state_cmp in Hdummy.
 discriminate.
 Qed.
 
+
+
+(* sv1 sv2 maxidx1 sb1 maxid2 sb2 instk_height ops -> bool *)
+Definition sstack_val_cmp_t := sstack_val -> sstack_val -> nat -> sbindings -> nat -> sbindings -> nat -> stack_op_instr_map -> bool.
+
+(* sstack_val_cmp smem1 smem2 maxidx1 sb1 maxid2 sb2 instk_height ops -> bool *)
+Definition smemory_cmp_t := sstack_val_cmp_t -> smemory -> smemory -> nat -> sbindings -> nat -> sbindings -> nat -> stack_op_instr_map -> bool.
+
+(* sstack_val_cmp sstrg1 sstrg2 maxidx1 sb1 maxid2 sb2 instk_height ops -> bool *)
+Definition sstorage_cmp_t := sstack_val_cmp_t -> sstorage -> sstorage -> nat -> sbindings -> nat -> sbindings -> nat -> stack_op_instr_map -> bool.
+
+(* sstack_val_cmp smemory_cmp soffset1 ssize1 smem1 soffset2 ssize2 smem2 maxidx1 sb1 maxid2 sb2 instk_height ops -> bool *)
+Definition sha3_cmp_t  := sstack_val_cmp_t -> sstack_val -> sstack_val -> smemory -> sstack_val -> sstack_val -> smemory -> nat -> sbindings -> nat -> sbindings -> nat -> stack_op_instr_map -> bool.
+
+Definition sstack_val_cmp_ext_1_t := nat -> sstack_val_cmp_t.
+
+Definition sstack_val_cmp_ext_2_t := smemory_cmp_t -> sstorage_cmp_t -> sha3_cmp_t -> sstack_val_cmp_ext_1_t.
+
+
+
+Definition make_sstack_val_cmp (sstack_value_cmp: sstack_val_cmp_ext_1_t) (d :nat) :=
+  (fun sv1 sv2 maxidx1 sb1 maxidx2 sb2 instk_height ops => sstack_value_cmp d sv1 sv2 maxidx1 sb1 maxidx2 sb2 instk_height ops).
+
+Definition make_sstack_val_cmp_ext_1 (smemory_cmp: smemory_cmp_t) (sstorage_cmp: sstorage_cmp_t) (sha3_cmp: sha3_cmp_t) (sstack_value_cmp: sstack_val_cmp_ext_2_t) :=
+  (fun d sv1 sv2 maxidx1 sb1 maxidx2 sb2 instk_height ops => sstack_value_cmp smemory_cmp sstorage_cmp sha3_cmp d sv1 sv2 maxidx1 sb1 maxidx2 sb2 instk_height ops).
+
+
+Definition safe_smemory_cmp_d (smemory_cmp: smemory_cmp_t) (sstack_val_cmp: sstack_val_cmp_ext_1_t) (d: nat) :=
+  forall smem1 smem2 maxidx1 sb1 maxidx2 sb2 instk_height ops,
+    valid_bindings instk_height maxidx1 sb1 ops ->
+    valid_bindings instk_height maxidx2 sb2 ops ->
+    valid_smemory instk_height maxidx1 smem1 ->
+    valid_smemory instk_height maxidx2 smem2 ->
+    smemory_cmp (make_sstack_val_cmp sstack_val_cmp d) smem1 smem2 maxidx1 sb1 maxidx2 sb2 instk_height ops = true ->
+    forall stk mem strg ctx,
+      exists mem',
+           eval_smemory smem1 maxidx1 sb1 stk mem strg ctx ops = Some mem' /\
+             eval_smemory smem1 maxidx1 sb1 stk mem strg ctx ops = Some mem'.
+
+Definition safe_sstorage_cmp_d (sstorage_cmp: sstorage_cmp_t) (sstack_val_cmp: sstack_val_cmp_ext_1_t) (d: nat) :=
+  forall sstrg1 sstrg2 maxidx1 sb1 maxidx2 sb2 instk_height ops,
+    valid_bindings instk_height maxidx1 sb1 ops ->
+    valid_bindings instk_height maxidx2 sb2 ops ->
+    valid_sstorage instk_height maxidx1 sstrg1 ->
+    valid_sstorage instk_height maxidx2 sstrg2 ->
+    sstorage_cmp (make_sstack_val_cmp sstack_val_cmp d) sstrg1 sstrg2 maxidx1 sb1 maxidx2 sb2 instk_height ops = true ->
+    forall stk mem strg ctx,
+    exists strg',
+      eval_sstorage sstrg1 maxidx1 sb1 stk mem strg ctx ops = Some strg' /\
+        eval_sstorage sstrg1 maxidx1 sb1 stk mem strg ctx ops = Some strg'.
+
+Definition safe_sha3_cmp_d (sha3_cmp: sha3_cmp_t) (sstack_val_cmp: sstack_val_cmp_ext_1_t) (d: nat) :=
+  forall soffset1 ssize1 smem1 soffset2 ssize2 smem2 maxidx1 sb1 maxidx2 sb2 instk_height ops,
+    valid_sstack_value instk_height maxidx1 soffset1 ->
+    valid_sstack_value instk_height maxidx1 ssize1 ->
+    valid_sstack_value instk_height maxidx2 soffset2 ->
+    valid_sstack_value instk_height maxidx2 ssize2 ->
+    valid_bindings instk_height maxidx1 sb1 ops ->
+    valid_bindings instk_height maxidx2 sb2 ops ->
+    valid_smemory instk_height maxidx1 smem1 ->
+    valid_smemory instk_height maxidx2 smem2 ->
+    sha3_cmp (make_sstack_val_cmp sstack_val_cmp d) soffset1 ssize1 smem1 soffset2 ssize2 smem2 maxidx1 sb1 maxidx2 sb2 instk_height ops = true ->
+    forall stk mem strg ctx,
+      exists offset1 size1 mem1 offset2 size2 mem2,
+      eval_smemory smem1 maxidx1 sb1 stk mem strg ctx ops = Some mem1 /\
+      eval_smemory smem1 maxidx1 sb1 stk mem strg ctx ops = Some mem2 /\
+      eval_sstack_val soffset1 stk mem strg ctx maxidx1 sb1 ops = Some offset1 /\
+      eval_sstack_val ssize1 stk mem strg ctx maxidx1 sb1 ops = Some size1 /\
+      eval_sstack_val soffset2 stk mem strg ctx maxidx1 sb1 ops = Some offset2 /\
+      eval_sstack_val ssize2 stk mem strg ctx maxidx1 sb1 ops = Some size2 /\
+      (get_keccak256_ctx ctx) (wordToNat size1) (mload' mem1 offset1 (wordToNat size1)) =
+      (get_keccak256_ctx ctx) (wordToNat size2) (mload' mem2 offset2 (wordToNat size2)).
+
+Definition safe_sstack_val_cmp_ext_2_d (smemory_cmp: smemory_cmp_t) (sstorage_cmp: sstorage_cmp_t) (sha3_cmp: sha3_cmp_t) (sstack_val_cmp: sstack_val_cmp_ext_2_t) (d: nat) :=
+  forall sv1 sv2 maxidx1 sb1 maxidx2 sb2 instk_height ops,
+    valid_sstack_value instk_height maxidx1 sv1 ->
+    valid_sstack_value instk_height maxidx2 sv2 ->
+    valid_bindings instk_height maxidx1 sb1 ops ->
+    valid_bindings instk_height maxidx2 sb2 ops ->
+    sstack_val_cmp smemory_cmp sstorage_cmp sha3_cmp d sv1 sv2 maxidx1 sb1 maxidx2 sb2 instk_height ops = true ->
+    forall stk mem strg ctx,
+    exists v,
+      eval_sstack_val sv1 stk mem strg ctx maxidx1 sb1 ops = Some v /\
+      eval_sstack_val sv2 stk mem strg ctx maxidx2 sb2 ops = Some v.
+
+
+Definition safe_smemory_cmp (smemory_cmp: smemory_cmp_t) (sstack_val_cmp: sstack_val_cmp_ext_1_t) :=
+  forall d, safe_smemory_cmp_d smemory_cmp sstack_val_cmp d.
+
+Definition safe_sstorage_cmp (sstorage_cmp: sstorage_cmp_t) (sstack_val_cmp: sstack_val_cmp_ext_1_t) :=
+  forall d, safe_sstorage_cmp_d sstorage_cmp sstack_val_cmp d.
+
+Definition safe_sha3_cmp (sha3_cmp: sha3_cmp_t) (sstack_val_cmp: sstack_val_cmp_ext_1_t) :=
+  forall d, safe_sha3_cmp_d sha3_cmp sstack_val_cmp d.
+
+Definition safe_sstack_val_cmp_ext_2 (smemory_cmp: smemory_cmp_t) (sstorage_cmp: sstorage_cmp_t) (sha3_cmp: sha3_cmp_t) (sstack_val_cmp: sstack_val_cmp_ext_2_t) :=
+  forall d, safe_sstack_val_cmp_ext_2_d smemory_cmp sstorage_cmp sha3_cmp sstack_val_cmp d.
+
+Definition safe_smemory_cmp_wrt_sstack_value_cmp (smemory_cmp: smemory_cmp_t) (sstorage_cmp: sstorage_cmp_t) (sha3_cmp: sha3_cmp_t) (sstack_val_cmp: sstack_val_cmp_ext_2_t) :=
+  forall d,
+    safe_sstack_val_cmp_ext_2_d smemory_cmp sstorage_cmp sha3_cmp sstack_val_cmp d ->
+    safe_smemory_cmp_d smemory_cmp (make_sstack_val_cmp_ext_1 smemory_cmp sstorage_cmp sha3_cmp sstack_val_cmp) d.
+
+Definition safe_sstorage_cmp_wrt_sstack_value_cmp (smemory_cmp: smemory_cmp_t) (sstorage_cmp: sstorage_cmp_t) (sha3_cmp: sha3_cmp_t) (sstack_val_cmp: sstack_val_cmp_ext_2_t) :=
+  forall d,
+    safe_sstack_val_cmp_ext_2_d smemory_cmp sstorage_cmp sha3_cmp sstack_val_cmp d ->
+    safe_sstorage_cmp_d sstorage_cmp (make_sstack_val_cmp_ext_1 smemory_cmp sstorage_cmp sha3_cmp sstack_val_cmp) d.
+
+Definition safe_sha3_cmp_wrt_sstack_value_cmp (smemory_cmp: smemory_cmp_t) (sstorage_cmp: sstorage_cmp_t) (sha3_cmp: sha3_cmp_t) (sstack_val_cmp: sstack_val_cmp_ext_2_t) :=
+  forall d,
+    safe_sstack_val_cmp_ext_2_d smemory_cmp sstorage_cmp sha3_cmp sstack_val_cmp d ->
+    safe_sha3_cmp_d sha3_cmp (make_sstack_val_cmp_ext_1 smemory_cmp sstorage_cmp sha3_cmp sstack_val_cmp) d.
+
+Definition safe_sstack_value_cmp_wrt_others (smemory_cmp: smemory_cmp_t) (sstorage_cmp: sstorage_cmp_t) (sha3_cmp: sha3_cmp_t) (sstack_val_cmp: sstack_val_cmp_ext_2_t) :=
+  forall d,
+    safe_smemory_cmp_d smemory_cmp (make_sstack_val_cmp_ext_1 smemory_cmp sstorage_cmp sha3_cmp sstack_val_cmp) d ->
+    safe_sstorage_cmp_d sstorage_cmp (make_sstack_val_cmp_ext_1 smemory_cmp sstorage_cmp sha3_cmp sstack_val_cmp) d ->
+    safe_sha3_cmp_d sha3_cmp (make_sstack_val_cmp_ext_1 smemory_cmp sstorage_cmp sha3_cmp sstack_val_cmp) d ->
+    safe_sstack_val_cmp_ext_2_d smemory_cmp sstorage_cmp sha3_cmp sstack_val_cmp (S d).
+
+Lemma safe_gh:
+  forall (smemory_cmp: smemory_cmp_t) (sstorage_cmp: sstorage_cmp_t) (sha3_cmp: sha3_cmp_t) (sstack_val_cmp: sstack_val_cmp_ext_2_t),
+    safe_smemory_cmp_wrt_sstack_value_cmp smemory_cmp sstorage_cmp sha3_cmp sstack_val_cmp ->
+    safe_sstorage_cmp_wrt_sstack_value_cmp smemory_cmp sstorage_cmp sha3_cmp sstack_val_cmp ->
+    safe_sha3_cmp_wrt_sstack_value_cmp smemory_cmp sstorage_cmp sha3_cmp sstack_val_cmp ->
+    safe_sstack_value_cmp_wrt_others smemory_cmp sstorage_cmp sha3_cmp sstack_val_cmp ->
+    safe_smemory_cmp smemory_cmp (make_sstack_val_cmp_ext_1 smemory_cmp sstorage_cmp sha3_cmp sstack_val_cmp) /\
+    safe_sstorage_cmp sstorage_cmp (make_sstack_val_cmp_ext_1 smemory_cmp sstorage_cmp sha3_cmp sstack_val_cmp) /\
+    safe_sha3_cmp sha3_cmp (make_sstack_val_cmp_ext_1 smemory_cmp sstorage_cmp sha3_cmp sstack_val_cmp) /\
+      safe_sstack_val_cmp_ext_2  smemory_cmp sstorage_cmp sha3_cmp sstack_val_cmp.
+Proof.
+Admitted.
+
 End SymbolicStateCmp.
 
   
