ver2/symbolic_state_cmp_impl.v
@@ -1,0 +1,152 @@
+Require Import Arith.
+Require Import Nat.
+Require Import Bool.
+Require Import bbv.Word.
+Require Import Coq.NArith.NArith.
+Require Import List.
+Import ListNotations.
+
+Require Import FORVES.constants.
+Import Constants.
+
+Require Import FORVES.program.
+Import Program.
+
+Require Import FORVES.execution_state.
+Import ExecutionState.
+
+Require Import FORVES.stack_operation_instructions.
+Import StackOpInstrs.
+
+Require Import FORVES.misc.
+Import Misc.
+
+Require Import FORVES.symbolic_state.
+Import SymbolicState.
+
+Require Import FORVES.symbolic_state_eval.
+Import SymbolicStateEval.
+
+
+Require Import FORVES.valid_symbolic_state.
+Import ValidSymbolicState.
+
+Require Import FORVES.valid_symbolic_state.
+Import ValidSymbolicState.
+
+Require Import FORVES.symbolic_state_cmp.
+Import SymbolicStateCmp.
+
+Require Import FORVES.eval_common.
+Import EvalCommon.
+
+Module SymbolicStateCmpImp.
+
+
+Fixpoint comapre_sstack_val (smemory_cmp: smemory_cmp_t) (sstorage_cmp: sstorage_cmp_t) (sha3_cmp: sha3_cmp_t) (d: nat) (sv1 sv2: sstack_val) (maxidx1: nat) (sb1: sbindings) (maxidx2: nat) (sb2: sbindings) (instk_height: nat) (ops: stack_op_instr_map) : bool :=
+  match d with
+  | 0 => false
+  | S d' =>
+      let comapre_sstack_val_rec :=
+        fun (sv1 sv2: sstack_val) (maxidx1: nat) (sb1: sbindings) (maxidx2: nat) (sb2: sbindings) (instk_height: nat) (ops: stack_op_instr_map) =>
+          comapre_sstack_val smemory_cmp sstorage_cmp sha3_cmp d' sv1 sv2 maxidx1 sb1 maxidx2 sb2 instk_height ops in
+      match follow_in_smap sv1 maxidx1 sb1, follow_in_smap sv2 maxidx2 sb2 with
+      | Some (FollowSmapVal smv1 maxidx1' sb1'), Some (FollowSmapVal smv2 maxidx2' sb2') =>
+          match smv1, smv2 with
+          | SymBasicVal (Val w1), SymBasicVal (Val w2) => weqb w1 w2
+          | SymBasicVal (InStackVar n1), SymBasicVal (InStackVar n2) => (andb (n1 =? n2) (andb (n1 <? instk_height) (n2 <? instk_height)))
+          | SymPUSHTAG v1, SymPUSHTAG v2 => (v1 =? v2)%N
+          | SymOp label1 args1, SymOp label2 args2 =>
+              if label1 =?i label2 then
+                match ops label1 with
+                  OpImp _ _ H_Comm _ =>
+                    match (fold_right_two_lists (fun e1 e2 => comapre_sstack_val_rec e1 e2 maxidx1' sb1' maxidx2' sb2' instk_height ops) args1 args2) with
+                    | true => true
+                    | false =>
+                        match H_Comm with
+                        | Some comm_proof =>
+                            match args1, args2 with
+                            | [a1;a2],[b1;b2] =>
+                                if comapre_sstack_val_rec a1 b2 maxidx1' sb1' maxidx2' sb2' instk_height ops
+                                then comapre_sstack_val_rec a2 b1 maxidx1' sb1' maxidx2' sb2' instk_height ops
+                                else false
+                            | _, _ => false
+                            end
+                        | None => false
+                        end
+                    end
+                end
+              else false
+          | SymMLOAD soffset1 smem1, SymMLOAD soffset2 smem2 =>
+              if comapre_sstack_val smemory_cmp sstorage_cmp sha3_cmp d' soffset1 soffset2 maxidx1' sb1' maxidx2' sb2' instk_height ops
+              then smemory_cmp comapre_sstack_val_rec smem1 smem2 maxidx1' sb1' maxidx2' sb2' instk_height ops
+              else false
+          | SymSLOAD skey1 sstrg1, SymSLOAD skey2 sstrg2 => 
+              if comapre_sstack_val smemory_cmp sstorage_cmp sha3_cmp d' skey1 skey2 maxidx1' sb1' maxidx2' sb2' instk_height ops
+              then sstorage_cmp comapre_sstack_val_rec sstrg1 sstrg2 maxidx1' sb1' maxidx2' sb2' instk_height ops
+              else false
+          | SymSHA3 soffset1 ssize1 smem1, SymSHA3 soffset2 ssize2 smem2 =>
+              (* the nested if is to avoid using band *)
+              if (if comapre_sstack_val_rec soffset1 soffset2 maxidx1' sb1' maxidx2' sb2' instk_height ops then
+                    if comapre_sstack_val_rec ssize1 ssize2 maxidx1' sb1' maxidx2' sb2' instk_height ops then
+                      if smemory_cmp comapre_sstack_val_rec smem1 smem2 maxidx1' sb1' maxidx2' sb2' instk_height ops then
+                        true
+                      else
+                        false
+                    else
+                      false
+                  else
+                    false)
+              then true
+              else sha3_cmp comapre_sstack_val_rec soffset1 ssize1 smem1 soffset2 ssize2 smem2 maxidx1' sb1' maxidx2' sb2' instk_height ops
+
+          | _, _ => false
+          end
+      | _, _ => false
+      end
+  end.
+
+
+Definition compare_sstack (smemory_cmp: smemory_cmp_t) (sstorage_cmp: sstorage_cmp_t) (sha3_cmp: sha3_cmp_t) (d: nat) (sstk1 sstk2: sstack) (maxidx1: nat) (sb1: sbindings) (maxidx2: nat) (sb2: sbindings) (instk_height: nat) (ops: stack_op_instr_map) : bool :=
+  fold_right_two_lists (fun e1 e2 => comapre_sstack_val smemory_cmp sstorage_cmp sha3_cmp d e1 e2 maxidx1 sb1 maxidx2 sb2 instk_height ops) sstk1 sstk2.
+
+Definition compare_smemory (smemory_cmp: smemory_cmp_t) (sstorage_cmp: sstorage_cmp_t) (sha3_cmp: sha3_cmp_t) (d: nat) (smem1 smem2: smemory) (maxidx1: nat) (sb1: sbindings) (maxidx2: nat) (sb2: sbindings) (instk_height: nat) (ops: stack_op_instr_map) : bool :=
+      let comapre_sstack_val_rec :=
+        fun (sv1 sv2: sstack_val) (maxidx1: nat) (sb1: sbindings) (maxidx2: nat) (sb2: sbindings) (instk_height: nat) (ops: stack_op_instr_map) =>
+          comapre_sstack_val smemory_cmp sstorage_cmp sha3_cmp d sv1 sv2 maxidx1 sb1 maxidx2 sb2 instk_height ops in
+      smemory_cmp comapre_sstack_val_rec smem1 smem2 maxidx1 sb1 maxidx2 sb2 instk_height ops.
+
+Definition compare_sstorage (smemory_cmp: smemory_cmp_t) (sstorage_cmp: sstorage_cmp_t) (sha3_cmp: sha3_cmp_t) (d: nat) (sstrg1 sstrg2: sstorage) (maxidx1: nat) (sb1: sbindings) (maxidx2: nat) (sb2: sbindings) (instk_height: nat) (ops: stack_op_instr_map) : bool :=
+      let comapre_sstack_val_rec :=
+        fun (sv1 sv2: sstack_val) (maxidx1: nat) (sb1: sbindings) (maxidx2: nat) (sb2: sbindings) (instk_height: nat) (ops: stack_op_instr_map) =>
+          comapre_sstack_val smemory_cmp sstorage_cmp sha3_cmp d sv1 sv2 maxidx1 sb1 maxidx2 sb2 instk_height ops in
+      sstorage_cmp comapre_sstack_val_rec sstrg1 sstrg2 maxidx1 sb1 maxidx2 sb2 instk_height ops.
+
+
+Definition sstate_cmp (smemory_cmp: smemory_cmp_t) (sstorage_cmp: sstorage_cmp_t) (sha3_cmp: sha3_cmp_t) (sst1 sst2: sstate) (ops: stack_op_instr_map) : bool :=
+  let instk_height1 := get_instk_height_sst sst1 in
+  let sstk1 := get_stack_sst sst1 in
+  let smem1 := get_memory_sst sst1 in 
+  let sstrg1 := get_storage_sst sst1 in
+  let m1 := get_smap_sst sst1 in
+  let maxidx1 := get_maxidx_smap m1 in
+  let sb1 := get_bindings_smap m1 in
+  let instk_height2 := get_instk_height_sst sst2 in
+  let sstk2 := get_stack_sst sst2 in
+  let smem2 := get_memory_sst sst2 in 
+  let sstrg2 := get_storage_sst sst2 in
+  let m2 := get_smap_sst sst2 in
+  let maxidx2 := get_maxidx_smap m2 in
+  let sb2 := get_bindings_smap m2 in
+  let d := S (max maxidx1 maxidx2) in
+  if instk_height1 =? instk_height1 then
+    if compare_sstack smemory_cmp sstorage_cmp sha3_cmp d sstk1 sstk2 maxidx1 sb1 maxidx2 sb2 instk_height1 ops then
+      if compare_smemory smemory_cmp sstorage_cmp sha3_cmp d smem1 smem2 maxidx1 sb1 maxidx2 sb2 instk_height1 ops then
+        if compare_sstorage smemory_cmp sstorage_cmp sha3_cmp d sstrg1 sstrg2 maxidx1 sb1 maxidx2 sb2 instk_height1 ops then
+          true
+        else false
+      else false
+    else false
+  else false.
+
+End SymbolicStateCmpImp.
